Hid states inside Automata

lean4/Automaton/DFA/Basic.lean
@@ -26,24 +26,24 @@ import Automaton.Fintype.List
 namespace DFA
 
 
-structure DFA (σs : Finset σ) (qs : Finset q) where
-  q₀ : qs           -- initial state
+structure DFA (σs : Finset σ) (q : Type _) where
+  qs : Finset q    -- set of states
+  q₀ : qs          -- initial state
   fs : Finset qs   -- accepting states
   δ : qs → σs → qs -- transition function
 
 
-variable {σ : Type _} {q : Type _}  {σs : Finset σ} {qs : Finset q} [DecidableEq σ] [DecidableEq q] (r s t : DFA σs qs)
-
+variable {σ : Type _} {q : Type _}  {σs : Finset σ}  [DecidableEq σ] [DecidableEq q] (r s t : DFA σs q)
 
 
 -- ToString
-instance instToString [ToString σ] [ToString q] [fσ : FinEnum σ] [fq : FinEnum q] : ToString (DFA σs qs) where
+instance instToString [ToString σ] [ToString q] [fσ : FinEnum σ] [fq : FinEnum q] : ToString (DFA σs q) where
   toString t := by
     have s : List String := (fσ.toList).map toString
     have q : String := toString t.q₀
     have qss : List String :=  (fq.toList).map toString
     have fs : List String := ((fq.toList).filter (fun e => e ∈ t.fs.map ⟨ fun a => a.1 , by simp [Function.Injective]⟩)).map toString
-    have δ : List String := (fq.toList).map (fun a => String.join ((fσ.toList).map (fun b => if h : a ∈ qs ∧ b ∈ σs then "("++ toString a ++ "×" ++ toString b ++ ")→" ++ toString (t.δ ⟨a , h.1⟩ ⟨b , h.2⟩) ++ " " else "")))
+    have δ : List String := (fq.toList).map (fun a => String.join ((fσ.toList).map (fun b => if h : a ∈ t.qs ∧ b ∈ σs then "("++ toString a ++ "×" ++ toString b ++ ")→" ++ toString (t.δ ⟨a , h.1⟩ ⟨b , h.2⟩) ++ " " else "")))
     exact "Σ: { " ++ String.join (s.map (fun e => e++" ")) ++ "}\n" ++
           "Q: { " ++ String.join (qss.map (fun e => e++" ")) ++ "}\n" ++
           "δ: " ++ String.join (δ.map (fun e => "\n   "++e)) ++ "\n" ++
@@ -55,12 +55,12 @@ instance instToString [ToString σ] [ToString q] [fσ : FinEnum σ] [fq : FinEnu
 -- the state reached after following all transitions given a word
 -- the first letter in list is the last character consumed
 @[simp]
-def δ_star' (q : qs) : (w : word σs) → qs
+def δ_star' (q : t.qs) : (w : word σs) → t.qs
   | [] => q
   | e :: es => δ_star' (t.δ q e) es
 
 
-def δ_star : (w : word σs) → qs := δ_star' t t.q₀
+def δ_star : (w : word σs) → t.qs := δ_star' t t.q₀
 
 -- whether a DFA accepts a word
 @[simp]
@@ -70,11 +70,11 @@ def dfaLang : Lang σs := fun w => dfa_accepts t w
 
 
 -- state is reachable from the given state
-inductive reachable (q : qs) : qs → Prop where
+inductive reachable (q : t.qs) : t.qs → Prop where
   | base : reachable q q
-  | step (q' : qs) : reachable q q' → ∀ e : σs , reachable q (t.δ q' e)
+  | step (q' : t.qs) : reachable q q' → ∀ e : σs , reachable q (t.δ q' e)
 
-theorem reachable_trans' (a b : qs) : reachable t a b → (c : qs) → reachable t b c → reachable t a c := by
+theorem reachable_trans' (a b : t.qs) : reachable t a b → (c : t.qs) → reachable t b c → reachable t a c := by
   intro h
   induction h with
   | base => intro c ac; exact ac
@@ -84,7 +84,7 @@ theorem reachable_trans' (a b : qs) : reachable t a b → (c : qs) → reachable
                      | base => apply reachable.step; exact reachable.base
                      | step q' _ e' s' => apply reachable.step; exact s'
 
-theorem reachable.trans (a b c : qs) : reachable t a b → reachable t b c → reachable t a c := by
+theorem reachable.trans (a b c : t.qs) : reachable t a b → reachable t b c → reachable t a c := by
   intro a
   apply reachable_trans'
   exact a
@@ -102,7 +102,7 @@ theorem dfa_accepts_nil_iff_final : dfa_accepts t [] ↔ t.q₀ ∈ t.fs := by
   <;> (first | simp [dfa_accepts])
   <;> exact h
 
-lemma δ_δ_star'_concat_eq_δ_star' : (q : qs) → DFA.δ t (δ_star' t q l) a = δ_star' t q (l ++ [a]) := by
+lemma δ_δ_star'_concat_eq_δ_star' : (q : t.qs) → DFA.δ t (δ_star' t q l) a = δ_star' t q (l ++ [a]) := by
   induction l with
   | nil => simp
   | cons e es s => intro q
@@ -118,7 +118,7 @@ theorem δ_star_append_eq (r : word σs) : (l : word σs) → δ_star t (l++r) =
                    simp [δ_star,δ_δ_star'_concat_eq_δ_star']
 
 
-theorem δ_star'_append_eq (r : word σs) (a : qs) : (l : word σs) → δ_star' t a (l++r) = δ_star' t (δ_star' t a l) r := by
+theorem δ_star'_append_eq (r : word σs) (a : t.qs) : (l : word σs) → δ_star' t a (l++r) = δ_star' t (δ_star' t a l) r := by
   induction r with
   | nil => simp
   | cons a as s => intro l
@@ -128,7 +128,7 @@ theorem δ_star'_append_eq (r : word σs) (a : qs) : (l : word σs) → δ_star'
 
 
 
-lemma δ_star'_reachable (w : word σs) (q : qs) : (q' : qs) → reachable t q q' → reachable t q (δ_star' t q' w) := by
+lemma δ_star'_reachable (w : word σs) (q : t.qs) : (q' : t.qs) → reachable t q q' → reachable t q (δ_star' t q' w) := by
   induction w with
   | nil => simp [δ_star]
   | cons e es s => intro q' rq'
@@ -137,13 +137,13 @@ lemma δ_star'_reachable (w : word σs) (q : qs) : (q' : qs) → reachable t q q
                    apply reachable.step
                    exact rq'
 
-theorem accepts_from_state_if (w : word σs) (q : qs) : (∀ q' : qs , (reachable t q q' → q' ∈ t.fs)) → δ_star' t q w ∈ t.fs := by
+theorem accepts_from_state_if (w : word σs) (q : t.qs) : (∀ q' : t.qs , (reachable t q q' → q' ∈ t.fs)) → δ_star' t q w ∈ t.fs := by
   intro q'
   apply q'
   apply δ_star'_reachable
   exact reachable.base
 
-theorem state_reachable_iff (q q' : qs) : reachable t q q' ↔ ∃ w : word σs , δ_star' t q w = q' := by
+theorem state_reachable_iff (q q' : t.qs) : reachable t q q' ↔ ∃ w : word σs , δ_star' t q w = q' := by
   apply Iff.intro
   · intro rq'
     induction rq' with
@@ -185,7 +185,7 @@ theorem ex_ne_nil_accepted_iff (h' : t.q₀ ∉ t.fs) : (∃ w, w ∈ dfaLang t 
     | inr h => exists w
 
 
-lemma reachable_δ_star' (w : word σs) (q : qs) : (q' : qs) → reachable t (δ_star' t q' w) q → reachable t q' q := by
+lemma reachable_δ_star' (w : word σs) (q : t.qs) : (q' : t.qs) → reachable t (δ_star' t q' w) q → reachable t q' q := by
   match w with
   | [] => simp
   | e::es => intro a r
@@ -197,7 +197,7 @@ lemma reachable_δ_star' (w : word σs) (q : qs) : (q' : qs) → reachable t (δ
              exists e :: es ++ w
 
 
-theorem accepts_prefix_if (l r : word σs) : (∀ q' : qs , (reachable t (δ_star t l) q' → q' ∈ t.fs)) → dfa_accepts t (l ++ r) := by
+theorem accepts_prefix_if (l r : word σs) : (∀ q' : t.qs , (reachable t (δ_star t l) q' → q' ∈ t.fs)) → dfa_accepts t (l ++ r) := by
   intro fa
   rw [dfa_accepts,δ_star_append_eq]
   apply accepts_from_state_if
@@ -208,7 +208,7 @@ theorem accepts_prefix_if (l r : word σs) : (∀ q' : qs , (reachable t (δ_sta
 -- To prove that DFA accepts any word starting with a prefix
 -- If after l, a state is reached from which all combinations of transitions lead
 -- to a final state, it always
-theorem accepts_prefix_iff (p : word σs) : (∀ s : word σs , dfa_accepts t (p ++ s)) ↔ dfa_accepts t p ∧ (∀ q' : qs , (reachable t (δ_star t p) q' → q' ∈ t.fs)) := by
+theorem accepts_prefix_iff (p : word σs) : (∀ s : word σs , dfa_accepts t (p ++ s)) ↔ dfa_accepts t p ∧ (∀ q' : t.qs , (reachable t (δ_star t p) q' → q' ∈ t.fs)) := by
   apply Iff.intro
   · intro h
     simp only [dfa_accepts] at h
@@ -227,7 +227,7 @@ theorem accepts_prefix_iff (p : word σs) : (∀ s : word σs , dfa_accepts t (p
     apply accepts_prefix_if
     apply h.2
 
-lemma accepts_suffix_if (l r : word σs) : (∀ q : qs , reachable t t.q₀ q → δ_star' t q r ∈ t.fs) → dfa_accepts t (l ++ r) := by
+lemma accepts_suffix_if (l r : word σs) : (∀ q : t.qs , reachable t t.q₀ q → δ_star' t q r ∈ t.fs) → dfa_accepts t (l ++ r) := by
   intro fa
   simp only [dfa_accepts]
   rw [δ_star_append_eq]
@@ -237,7 +237,7 @@ lemma accepts_suffix_if (l r : word σs) : (∀ q : qs , reachable t t.q₀ q �
 
 -- To prove that DFA always accepts some suffix
 -- If from any reachable state the word is accepted, it is always accepted
-theorem accepts_suffix_iff (s : word σs) : (∀ p : word σs,  dfa_accepts t (p ++ s)) ↔ (∀ q : qs , reachable t t.q₀ q → δ_star' t q s ∈ t.fs) := by
+theorem accepts_suffix_iff (s : word σs) : (∀ p : word σs,  dfa_accepts t (p ++ s)) ↔ (∀ q : t.qs , reachable t t.q₀ q → δ_star' t q s ∈ t.fs) := by
   apply Iff.intro
   · intro fa q rq
     have := Iff.mp (state_reachable_iff t t.q₀ q) rq
@@ -254,12 +254,12 @@ theorem accepts_suffix_iff (s : word σs) : (∀ p : word σs,  dfa_accepts t (p
 -- Define whether list forms path between start and finish
 -- The elements (vertices) are joined by edges and each vertex exists at most once
 -- The last element must be the target
-def is_path (a z : qs) : List qs → Prop
+def is_path (a z : t.qs) : List t.qs → Prop
   | [] => a = z
   | q :: qs => (∃ e : σs , t.δ a e = q) ∧ is_path q z qs ∧ q ∉ qs
 
 
-theorem target_in_path  (l : List qs) : (a b : qs) → is_path t a b l → a ≠ b → b ∈ l := by
+theorem target_in_path  (l : List t.qs) : (a b : t.qs) → is_path t a b l → a ≠ b → b ∈ l := by
   induction l with
   | nil => intro a b pab _; simp [is_path] at pab; contradiction
   | cons e es s => intro a b pab _;
@@ -277,7 +277,7 @@ theorem target_in_path  (l : List qs) : (a b : qs) → is_path t a b l → a ≠
                               apply h
                               rw [eq]
 
-lemma all_in_path_reachable (l : List qs) : (a b : qs) → is_path t a b l → ∀ q : qs, q ∈ l → reachable t a q := by
+lemma all_in_path_reachable (l : List t.qs) : (a b : t.qs) → is_path t a b l → ∀ q : t.qs, q ∈ l → reachable t a q := by
   induction l with
   | nil => intro a b _ q qin; contradiction
   | cons e es s => intro a b p q qinees
@@ -330,7 +330,7 @@ def nin_list_nin_list_until {α : Type _} [DecidableEq α] (a : α) (l : List α
                         · exact ain
 
 
-lemma path_if_list_until (l : List qs) : (a b : qs) → is_path t a b l → ∀ q : qs, q ∈ l → is_path t a q (list_until q l) := by
+lemma path_if_list_until (l : List t.qs) : (a b : t.qs) → is_path t a b l → ∀ q : t.qs, q ∈ l → is_path t a q (list_until q l) := by
   induction l with
   | nil => intro a b _ q qin; contradiction
   | cons e es s => intro a b pab q qin
@@ -359,7 +359,7 @@ lemma path_if_list_until (l : List qs) : (a b : qs) → is_path t a b l → ∀ 
 
 
 
-lemma all_in_path_path (l : List qs) : (a b : qs) → is_path t a b l → ∀ q : qs, q ∈ l → ∃ l₁ : List qs, is_path t a q l₁ := by
+lemma all_in_path_path (l : List t.qs) : (a b : t.qs) → is_path t a b l → ∀ q : t.qs, q ∈ l → ∃ l₁ : List t.qs, is_path t a q l₁ := by
   match l with
   | [] => intro a b _ q qin; contradiction
   | e::es => intro a b p q qin
@@ -369,7 +369,7 @@ lemma all_in_path_path (l : List qs) : (a b : qs) → is_path t a b l → ∀ q 
              · exact qin
 
 
-lemma path_concat (l : List qs) : (a b c : qs) → is_path t a b l → (∃ e : σs, t.δ b e = c) → c ∉ l → is_path t a c (l.concat c) := by
+lemma path_concat (l : List t.qs) : (a b c : t.qs) → is_path t a b l → (∃ e : σs, t.δ b e = c) → c ∉ l → is_path t a c (l.concat c) := by
   induction l with
   | nil => intro a b c p ex cin
            simp only [is_path]
@@ -400,7 +400,7 @@ lemma path_concat (l : List qs) : (a b c : qs) → is_path t a b l → (∃ e : 
                          contradiction
 
 
-theorem reachable_iff_ex_path (a b : qs) : reachable t a b ↔ ∃ l : List qs , is_path t a b l := by
+theorem reachable_iff_ex_path (a b : t.qs) : reachable t a b ↔ ∃ l : List t.qs , is_path t a b l := by
   apply Iff.intro
   . intro r
     induction r with
@@ -431,7 +431,7 @@ theorem reachable_iff_ex_path (a b : qs) : reachable t a b ↔ ∃ l : List qs ,
 
 
 
-theorem path_nodup (l : List qs) : (a b : qs) → is_path t a b l → l.Nodup := by
+theorem path_nodup (l : List t.qs) : (a b : t.qs) → is_path t a b l → l.Nodup := by
   induction l with
   | nil => simp
   | cons e es s => intro a b h
@@ -442,13 +442,13 @@ theorem path_nodup (l : List qs) : (a b : qs) → is_path t a b l → l.Nodup :=
                    · apply s
                      · exact h.2.1
 
-lemma path_finset_subset (l : List qs) : (a b : qs) → is_path t a b l → l.toFinset ⊆ qs.attach := by
+lemma path_finset_subset (l : List t.qs) : (a b : t.qs) → is_path t a b l → l.toFinset ⊆ t.qs.attach := by
   intro a b _
   simp only [· ⊆ · ]
   intro e _
   apply Finset.mem_attach
 
-theorem path_le_size (l : List qs) : (a b : qs) → is_path t a b l → l.length ≤ qs.card := by
+theorem path_le_size (l : List t.qs) : (a b : t.qs) → is_path t a b l → l.length ≤ t.qs.card := by
   intro a b pab
   rw [←Finset.card_attach,←List.toFinset_card_of_nodup]
   apply Finset.card_le_of_subset
@@ -458,7 +458,7 @@ theorem path_le_size (l : List qs) : (a b : qs) → is_path t a b l → l.length
   exact pab
 
 
-theorem w_le_card_if_ex_w  (p : word qs) : (a b : qs) → is_path t a b p → (∃ w : word σs, δ_star' t a w = b ∧ w.length = p.length) := by
+theorem w_le_card_if_ex_w  (p : word t.qs) : (a b : t.qs) → is_path t a b p → (∃ w : word σs, δ_star' t a w = b ∧ w.length = p.length) := by
   induction p with
   | nil => intro a b p
            exists []
@@ -478,7 +478,7 @@ theorem w_le_card_if_ex_w  (p : word qs) : (a b : qs) → is_path t a b p → (�
                    · rfl
 
 
-theorem ex_w_iff_ex_w_le_card (a b : qs) : (∃ w : word σs, δ_star' t a w = b) ↔ (∃ w : word σs, δ_star' t a w = b ∧ w.length <= qs.card) := by
+theorem ex_w_iff_ex_w_le_card (a b : t.qs) : (∃ w : word σs, δ_star' t a w = b) ↔ (∃ w : word σs, δ_star' t a w = b ∧ w.length <= t.qs.card) := by
   apply Iff.intro
   · intro ex
     have := (state_reachable_iff t a b).mpr ex
@@ -500,7 +500,7 @@ theorem ex_w_iff_ex_w_le_card (a b : qs) : (∃ w : word σs, δ_star' t a w = b
     exists w
     exact h.1
 
-instance DecidableExW {P : word σs → Prop} [f : Fintype {x : word σs // x.length <= qs.card}] [DecidablePred P] : Decidable (∃ w : {x : word σs // x.length <= qs.card}, P w ) := by
+instance DecidableExW {P : word σs → Prop} [f : Fintype {x : word σs // x.length <= t.qs.card}] [DecidablePred P] : Decidable (∃ w : {x : word σs // x.length <= t.qs.card}, P w ) := by
   have h : Decidable (∃ l, l ∈ f.elems ∧ (fun l => P l) l) := Finset.decidableExistsAndFinset
   match h with
   | isTrue t => apply isTrue
@@ -520,7 +520,7 @@ instance DecidableExW {P : word σs → Prop} [f : Fintype {x : word σs // x.le
 
 instance idk [Decidable a] [Decidable b] [Decidable c] : Decidable (a ∧ b ∧ c) := by infer_instance
 
-instance decIsPath : (a b : qs) → Decidable (is_path t a b w) := by
+instance decIsPath : (a b : t.qs) → Decidable (is_path t a b w) := by
   induction w with
   | nil => simp only [is_path]
            infer_instance
@@ -528,9 +528,9 @@ instance decIsPath : (a b : qs) → Decidable (is_path t a b w) := by
                  intro a b
                  infer_instance
 
-instance decExIsPath : (a b : qs) → Decidable (∃ l : List qs, is_path t a b l) := by
+instance decExIsPath : (a b : t.qs) → Decidable (∃ l : List t.qs, is_path t a b l) := by
   intro a b
-  have f : Fintype {p : List qs // p.Nodup} := fintypeNodupList
+  have f : Fintype {p : List t.qs // p.Nodup} := fintypeNodupList
   have h : Decidable (∃ l, l ∈ f.elems ∧ (fun l => is_path t a b l) l) := Finset.decidableExistsAndFinset
   match h with
   | isTrue t => apply isTrue
@@ -551,7 +551,7 @@ instance decExIsPath : (a b : qs) → Decidable (∃ l : List qs, is_path t a b 
 
 instance decReachable : DecidableRel (reachable t) := by
   intro a b
-  apply decidable_of_iff (∃ l : List qs, is_path t a b l)
+  apply decidable_of_iff (∃ l : List t.qs, is_path t a b l)
   apply Iff.symm
   apply reachable_iff_ex_path
 
