lean4/Automaton/NFA/ToDFA.lean
@@ -12,37 +12,38 @@ open NFA DFA Finset
 
 namespace ToDFA
 
-variable {σ : Type _} {q : Type _} {σs : Finset σ} {qs : Finset q} (r s tn : NFA σs qs) [DecidableEq σ] [DecidableEq q]
+variable {σ : Type _} {q : Type _} {σs : Finset σ} (r s tn : NFA σs q) [DecidableEq σ] [DecidableEq q]
 
 @[simp]
-def nfa_to_dfa_q : Finset (Finset qs) := qs.attach.powerset
+def nfa_to_dfa_q : Finset (Finset tn.qs) := tn.qs.attach.powerset
 
 @[simp]
-theorem all_in_q (q : Finset qs) : q ∈ nfa_to_dfa_q  := by
+theorem all_in_q (q : Finset tn.qs) : q ∈ nfa_to_dfa_q tn := by
   simp [nfa_to_dfa_q, · ⊆ ·]
 
 @[simp]
-def nfa_to_dfa_init : { x // x ∈ @nfa_to_dfa_q q qs } := ⟨tn.q₀ , all_in_q tn.q₀⟩
+def nfa_to_dfa_init : { x // x ∈ nfa_to_dfa_q tn } := ⟨tn.q₀ , all_in_q _ tn.q₀⟩
 
 @[simp]
-def nfa_to_dfa_fs : Finset { x // x ∈ @nfa_to_dfa_q q qs } :=
-  (nfa_to_dfa_q.filter (fun q => (q ∩ tn.fs).Nonempty)).map  ⟨(fun q => ⟨q , all_in_q  q⟩), by simp [Function.Injective]⟩
+def nfa_to_dfa_fs : Finset { x // x ∈ nfa_to_dfa_q tn } :=
+  ((nfa_to_dfa_q tn).filter (fun q => (q ∩ tn.fs).Nonempty)).map  ⟨(fun q => ⟨q , all_in_q tn q⟩), by simp [Function.Injective]⟩
 
 
-def nfa_to_dfa_δ : { x // x ∈ @nfa_to_dfa_q q qs } → σs → { x // x ∈ @nfa_to_dfa_q q qs } := by
+def nfa_to_dfa_δ : { x // x ∈ nfa_to_dfa_q tn } → σs → { x // x ∈ nfa_to_dfa_q tn } := by
   intro q e
-  exact ⟨q.1.biUnion (fun q => tn.δ q e) , all_in_q _⟩
+  exact ⟨q.1.biUnion (fun q => tn.δ q e) , all_in_q tn _⟩
 
-def nfa_to_dfa : DFA σs (@nfa_to_dfa_q q qs) :=
+def nfa_to_dfa : DFA σs (Finset tn.qs) :=
   {q₀ := nfa_to_dfa_init tn, fs := nfa_to_dfa_fs tn , δ := nfa_to_dfa_δ tn}
 
-theorem δ_star_eq' : (q : Finset qs) → ⟨(NFA.δ_star' tn q w) , all_in_q  (NFA.δ_star' tn q w)⟩ = DFA.δ_star' (nfa_to_dfa tn) ⟨ q , (all_in_q q)⟩  w := by
+
+theorem δ_star_eq' : (q : Finset tn.qs) → ⟨(NFA.δ_star' tn q w) , all_in_q tn _⟩ = DFA.δ_star' (nfa_to_dfa tn) ⟨q , (all_in_q tn q)⟩  w := by
   induction w with
   | nil => simp [NFA.δ_star,DFA.δ_star,nfa_to_dfa]
   | cons a as s => intro q
                    simp [NFA.δ_star,DFA.δ_star,s,nfa_to_dfa,nfa_to_dfa_δ,δ_step]
 
-theorem δ_star_eq : ⟨(NFA.δ_star tn w) , all_in_q (NFA.δ_star tn w)⟩ = DFA.δ_star (nfa_to_dfa tn) w := by
+theorem δ_star_eq : ⟨(NFA.δ_star tn w) , all_in_q tn (NFA.δ_star  tn w)⟩ = DFA.δ_star (nfa_to_dfa tn) w := by
   apply δ_star_eq'
 
 theorem nfa_to_dfa_eq (w : word σs) : nfa_accepts tn w ↔ dfa_accepts (nfa_to_dfa tn) w := by
